Equivalence implies trace bisimilarity
First draft of a proof, following the paper. "First draft" because the
proof is supremely ugly.

TraceEqualityEquivalence.v
@@ -1,5 +1,6 @@
-Require Import Contractive Equivalence Free SessionTypes Substitution
-  SubstitutionFacts Msg Tac TraceLanguage TraceLanguageFacts Var Wellformed.
+Require Import Contractive CompleteSubstitution CompleteSubstitutionFacts
+  Equivalence Free SessionTypes Substitution SubstitutionFacts Msg Tac
+  TraceLanguage TraceLanguageFacts Var Wellformed.
 
 
 Create HintDb tleq discriminated.
@@ -108,3 +109,119 @@ Unshelve.
     end;
     eauto with wf subst.
 Qed.
+
+
+Inductive R_equivalence_trace_bisim' : Tl -> Tl -> Prop :=
+| R_equivalence_trace_bisim'_intro :
+    forall l l' eta,
+    (exists S S' c c',
+     tl eta (cs S) c = l /\
+     tl eta (cs S') c' = l' /\
+     wellformed S /\
+     wellformed S' /\
+     sequiv (cs S) (cs S')
+    ) ->
+    R_equivalence_trace_bisim' l l'.
+
+
+(* TODO ouch *)
+Lemma equivalence_trace_bisim' :
+  forall S S' eta c c',
+  wellformed S ->
+  wellformed S' ->
+  sequiv S S' ->
+  Tl_bisim (tl eta S c) (tl eta S' c').
+Proof.
+  intros. (rewrite_strat (subterms cs_preserves_tl)); try assumption.
+  apply Tl_bisim_coind with (R := R_equivalence_trace_bisim').
+  - clear. introv CIH. inverts1 CIH. norm_hyp_auto.
+    rename H0 into Hwf. rename H2 into Hwf'. rename H4 into Hsequiv.
+    subst. inverts2 Hsequiv.
+    * gen c c' Hwf Hwf'. rewrite <- Hsequiv. rewrite <- H2.
+      clear Hsequiv. clear H2.
+      introv Hwf Hwf'. constructor.
+    * gen c c' Hwf Hwf'. rewrite <- H0. rewrite <- H1.
+      introv Hwf Hwf'.
+      assert (wellformed (send B S0)) as Htmp1 by (rewrite H0; auto with subst).
+      assert (wellformed (send B S'0)) as Htmp2 by (rewrite H1; auto with subst).
+      apply wellformed_inv in Htmp1. apply wellformed_inv in Htmp2.
+      simpl. constructor. econstructor.
+      exists S0 S'0. eexists. eexists. splits.
+      + symmetry. apply cs_preserves_tl. assumption.
+      + symmetry. apply cs_preserves_tl. assumption.
+      + assumption.
+      + assumption.
+      + apply cs_preserves_sequiv; eauto.
+    * gen c c' Hwf Hwf'. rewrite <- H0. rewrite <- H1.
+      introv Hwf Hwf'.
+      assert (wellformed (recv B S0)) as Htmp1 by (rewrite H0; auto with subst).
+      assert (wellformed (recv B S'0)) as Htmp2 by (rewrite H1; auto with subst).
+      apply wellformed_inv in Htmp1. apply wellformed_inv in Htmp2.
+      simpl. constructor. econstructor.
+      exists S0 S'0. eexists. eexists. splits.
+      + symmetry. apply cs_preserves_tl. assumption.
+      + symmetry. apply cs_preserves_tl. assumption.
+      + assumption.
+      + assumption.
+      + apply cs_preserves_sequiv; eauto.
+    * gen c c' Hwf Hwf'. rewrite <- H0. rewrite <- H1.
+      introv Hwf Hwf'.
+      assert (wellformed (echoice S1 S2)) as Htmp1 by (rewrite H0; auto with subst).
+      assert (wellformed (echoice S1' S2')) as Htmp2 by (rewrite H1; auto with subst).
+      apply wellformed_inv in Htmp1. apply wellformed_inv in Htmp2.
+      destruct Htmp1. destruct Htmp2.
+      simpl. constructor.
+      + econstructor. exists S1. exists S1'. eexists. eexists. splits.
+        -- symmetry. apply cs_preserves_tl. assumption.
+        -- symmetry. apply cs_preserves_tl. assumption.
+        -- assumption.
+        -- assumption.
+        -- apply cs_preserves_sequiv; eauto.
+      + econstructor. exists S2. exists S2'. eexists. eexists. splits.
+        -- symmetry. apply cs_preserves_tl. assumption.
+        -- symmetry. apply cs_preserves_tl. assumption.
+        -- assumption.
+        -- assumption.
+        -- apply cs_preserves_sequiv; eauto.
+    * gen c c' Hwf Hwf'. rewrite <- H0. rewrite <- H1.
+      introv Hwf Hwf'.
+      assert (wellformed (ichoice S1 S2)) as Htmp1 by (rewrite H0; auto with subst).
+      assert (wellformed (ichoice S1' S2')) as Htmp2 by (rewrite H1; auto with subst).
+      apply wellformed_inv in Htmp1. apply wellformed_inv in Htmp2.
+      destruct Htmp1. destruct Htmp2.
+      simpl. constructor.
+      + econstructor. exists S1. exists S1'. eexists. eexists. splits.
+        -- symmetry. apply cs_preserves_tl. assumption.
+        -- symmetry. apply cs_preserves_tl. assumption.
+        -- assumption.
+        -- assumption.
+        -- apply cs_preserves_sequiv; eauto.
+      + econstructor. exists S2. exists S2'. eexists. eexists. splits.
+        -- symmetry. apply cs_preserves_tl. assumption.
+        -- symmetry. apply cs_preserves_tl. assumption.
+        -- assumption.
+        -- assumption.
+        -- apply cs_preserves_sequiv; eauto.
+    * symmetry in H0. apply cs_mu_absurd in H0.
+      + contradiction.
+      + eauto with wf.
+    * symmetry in H0. apply cs_mu_absurd in H0.
+      + contradiction.
+      + eauto with wf.
+  - econstructor. exists S. exists S'. eexists. eexists. splits;
+    auto with subst.
+    * apply cs_preserves_sequiv; eauto with wf.
+Unshelve.
+  all:
+    try solve
+      [apply wellformed_Contractive; auto with subst].
+Qed.
+
+Theorem equivalence_trace_bisim :
+  forall S S' eta
+  (Swf : wellformed S)
+  (S'wf : wellformed S'),
+  sequiv S S' ->
+  Tl_bisim (tl eta S (wellformed_Contractive _ Swf))
+    (tl eta S' (wellformed_Contractive _ S'wf)).
+Proof. intros. apply equivalence_trace_bisim'; auto. Qed.
